Pushing through final updates for the day

lean_source/A_03_Recursive_Types/A_05_recursive_proofs.lean
@@ -8,3 +8,60 @@ Introduction
 
 Coming soon.
 TEXT. -/
+
+-- QUOTE:
+
+inductive le (n : nat): nat → Prop 
+-- n is an implicit firt argument to each constructor
+| refl : le /-n-/ n     
+| step : ∀ m, le /-n-/ m → le /-n-/ m.succ
+
+-- you can see it in the types of the constructors
+#check @le.refl
+#check @le.step
+
+
+example : le 0 0 :=
+begin
+apply le.refl,
+end 
+
+example : le 3 3 :=
+begin
+apply le.refl,
+end 
+
+example : le 0 1 :=
+begin
+apply le.step,
+apply le.refl,
+end 
+
+example : le 0 3 :=
+begin
+apply le.step,
+apply le.step,
+apply le.step,
+apply le.refl,
+end 
+
+
+-- here's the same example using Lean's version of "le"
+-- it's called nat.less_than_or_equal
+example : 0 ≤ 3 :=
+begin
+apply nat.less_than_or_equal.step,
+apply nat.less_than_or_equal.step,
+apply nat.less_than_or_equal.step,
+-- apply nat.less_than_or_equal.step,
+apply nat.less_than_or_equal.refl,
+end 
+
+-- repeat tactical goes too far; use iterate instead
+example : 1 ≤ 4 :=
+begin
+-- repeat {apply nat.less_than_or_equal.step},
+iterate 3 {apply nat.less_than_or_equal.step},
+apply nat.less_than_or_equal.refl,
+end 
+-- QUOTE.
